src/lib/collections/Collections.Seqs_i.fsti
@@ -16,11 +16,13 @@ val reverse_reverse_seq (#a:Type) (s:seq a) :
   Lemma(ensures reverse_seq (reverse_seq s) == s)
   [SMTPat (reverse_seq (reverse_seq s))]
 
+
 val seq_map_i_indexed (#a:Type) (#b:Type) (f:int->a->b) (s:seq a) (i:int) : 
   Tot (s':seq b { length s' == length s /\
                   (forall j . {:pattern index s' j} 0 <= j /\ j < length s ==> index s' j == f (i + j) (index s j))
                 }) 
-
+      (decreases %[(length s)])
+      
 val seq_map_i (#a:Type) (#b:Type) (f:int->a->b) (s:seq a) :
   Tot (s':seq b { length s' == length s /\
                   (forall j . {:pattern index s' j} 0 <= j /\ j < length s ==> index s' j == f j (index s j))
@@ -30,12 +32,6 @@ val seq_map_internal_associative (#a:Type) (#b:eqtype) (f:int->a->b) (s:seq a) (
   Lemma (let left,right = split s pivot in
          seq_map_i f s == seq_map_i_indexed f left 0 @| seq_map_i_indexed f right pivot )
 
-let seq_map_inverses (#a #b:Type) (f:a -> b) (g:b -> a) (s:seq a) : Lemma
+val seq_map_inverses (#a #b:Type) (f:a -> b) (g:b -> a) (s:seq a) : Lemma
   (requires forall x . g (f x) == x)
   (ensures seq_map g (seq_map f s) == s)
-  =
-  let mid = seq_map f s in
-  let final = seq_map g mid in
-  assert (equal s final);
-  ()
-  
